feat: remove the selector axiom (#1693)

scripts/check_axioms.py
@@ -26,7 +26,6 @@ LEAN_BUILTIN_AXIOMS = frozenset([
 ])
 
 DOCUMENTED_AXIOMS = frozenset([
-    "keccak256_first_4_bytes",
     "solidityMappingSlot_lt_evmModulus",
 ])
 
